Combine MessageHeader files
Combine contents of Definitions.dfy, Validity.dfy, and Utils.dfy into Format.dfy.
Combine contents of Serialize.dfy, SerializeAAD.dfy, and SerializeEDK.dfy into Serialize.dfy.
No other changes were made. In particular, this commit does not change the names of modules.

src/SDK/MessageHeader/Format.dfy
@@ -1,9 +1,77 @@
-include "Definitions.dfy"
-include "Utils.dfy"
-
+include "../AlgorithmSuite.dfy"
 include "../../StandardLibrary/StandardLibrary.dfy"
-include "../../Util/UTF8.dfy"
 include "../Materials.dfy"
+include "../../Util/Streams.dfy"
+include "../../Util/UTF8.dfy"
+
+module MessageHeader.Definitions {
+  import AlgorithmSuite
+  import opened StandardLibrary
+  import opened UInt = StandardLibrary.UInt
+  import Materials
+
+  /*
+   * Definition of the message header, i.e., the header body and the header authentication
+   */
+  datatype Header = Header(body: HeaderBody, auth: HeaderAuthentication)
+
+  /*
+   * Header body type definition
+   */
+  const VERSION_1: uint8     := 0x01
+  type Version               = x | x == VERSION_1 witness VERSION_1
+
+  const TYPE_CUSTOMER_AED: uint8 := 0x80
+  type Type                  = x | x == TYPE_CUSTOMER_AED witness TYPE_CUSTOMER_AED
+
+  const MESSAGE_ID_LEN       := 16
+  type MessageID             = x: seq<uint8> | |x| == MESSAGE_ID_LEN witness [0,0,0,0,0,0,0,0,0,0,0,0,0,0,0,0]
+
+  type Reserved              = x: seq<uint8> | x == [0,0,0,0] witness [0,0,0,0]
+
+  datatype ContentType       = NonFramed | Framed
+
+  function method ContentTypeToUInt8(contentType: ContentType): uint8 {
+    match contentType
+    case NonFramed => 0x01
+    case Framed => 0x02
+  }
+
+  function method UInt8ToContentType(x: uint8): Option<ContentType> {
+    if x == 0x01 then
+      Some(NonFramed)
+    else if x == 0x02 then
+      Some(Framed)
+    else
+      None
+  }
+
+  lemma ContentTypeConversionsCorrect(contentType: ContentType, x: uint8)
+    ensures UInt8ToContentType(ContentTypeToUInt8(contentType)) == Some(contentType)
+    ensures var opt := UInt8ToContentType(x); opt == None || ContentTypeToUInt8(opt.get) == x
+  {
+  }
+
+  datatype EncryptedDataKeys = EncryptedDataKeys(entries: seq<Materials.EncryptedDataKey>)
+
+  datatype HeaderBody        = HeaderBody(
+                                 version: Version,
+                                 typ: Type,
+                                 algorithmSuiteID: AlgorithmSuite.ID,
+                                 messageID: MessageID,
+                                 aad: Materials.EncryptionContext,
+                                 encryptedDataKeys: EncryptedDataKeys,
+                                 contentType: ContentType,
+                                 reserved: Reserved,
+                                 ivLength: uint8,
+                                 frameLength: uint32)
+
+  /*
+   * Header authentication type definition
+   */
+  datatype HeaderAuthentication = HeaderAuthentication(iv: seq<uint8>, authenticationTag: seq<uint8>)
+}
+
 
 module MessageHeader.Validity {
   import Msg = Definitions
@@ -184,5 +252,53 @@ module MessageHeader.Validity {
   {
     |ha.authenticationTag| == AlgorithmSuite.Suite[algorithmSuiteID].params.tagLen as int &&
     |ha.iv| == AlgorithmSuite.Suite[algorithmSuiteID].params.ivLen as int
+  }
+}
+
+
+module MessageHeader.Utils {
+  import AlgorithmSuite
+  import Streams
+  import opened StandardLibrary
+  import opened UInt = StandardLibrary.UInt
+
+  predicate SortedKVPairsUpTo(a: seq<(seq<uint8>, seq<uint8>)>, n: nat)
+    requires n <= |a|
+  {
+    forall j :: 0 < j < n ==> LexicographicLessOrEqual(a[j-1].0, a[j].0, UInt8Less)
+  }
+
+  predicate SortedKVPairs(a: seq<(seq<uint8>, seq<uint8>)>)
+  {
+    SortedKVPairsUpTo(a, |a|)
+  }
+
+  method InsertNewEntry(kvPairs: seq<(seq<uint8>, seq<uint8>)>, key: seq<uint8>, value: seq<uint8>)
+      returns (res: Option<seq<(seq<uint8>, seq<uint8>)>>, ghost insertionPoint: nat)
+    requires SortedKVPairs(kvPairs)
+    ensures match res
+    case None =>
+      exists i :: 0 <= i < |kvPairs| && kvPairs[i].0 == key  // key already exists
+    case Some(kvPairs') =>
+      && insertionPoint <= |kvPairs|
+      && kvPairs' == kvPairs[..insertionPoint] + [(key, value)] + kvPairs[insertionPoint..]
+      && SortedKVPairs(kvPairs')
+  {
+    var n := |kvPairs|;
+    while 0 < n && LexicographicLessOrEqual(key, kvPairs[n - 1].0, UInt8Less)
+      invariant 0 <= n <= |kvPairs|
+      invariant forall i :: n <= i < |kvPairs| ==> LexicographicLessOrEqual(key, kvPairs[i].0, UInt8Less)
+    {
+      n := n - 1;
+    }
+    if 0 < n && kvPairs[n - 1].0 == key {
+      return None, n;
+    } else {
+      var kvPairs' := kvPairs[..n] + [(key, value)] + kvPairs[n..];
+      if 0 < n {
+        LexPreservesTrichotomy(kvPairs'[n - 1].0, kvPairs'[n].0, UInt8Less);
+      }
+      return Some(kvPairs'), n;
+    }
   }
 }
